feat: Simple implementaiton

TestModels/resources/src/SimpleResourcesOperations.dfy
@@ -1,15 +1,16 @@
+// Copyright Amazon.com Inc. or its affiliates. All Rights Reserved.
+// SPDX-License-Identifier: Apache-2.0
+
 include "../Model/SimpleResourcesTypes.dfy"
+include "./Config.dfy"
+include "./SimpleResource.dfy"
 
-module SimpleResourcesImpl refines AbstractSimpleResourcesOperations {
-  datatype Config = Config
-  type InternalConfig = Config
+module SimpleResourcesOperations refines AbstractSimpleResourcesOperations {
+  import Config
+  import SimpleResource
 
-  predicate ValidInternalConfig?(config: InternalConfig)
-  {true}
-
-  function ModifiesInternalConfig(config: InternalConfig): set<object>
-  {{}}
-
+  type InternalConfig = Config.Config
+  
   predicate GetResourcesEnsuresPublicly(
     input: GetResourcesInput,
     output: Result<GetResourcesOutput, Error>
@@ -18,7 +19,26 @@ module SimpleResourcesImpl refines AbstractSimpleResourcesOperations {
   method GetResources(
     config: InternalConfig,
     input: GetResourcesInput
-  ) returns (output: Result<GetResourcesOutput, Error>)
-  
+  ) returns (
+    output: Result<GetResourcesOutput, Error>
+  )
+  {
+    :- Need(Config.ValidInternalConfig?(config),
+      Types.SimpleResourceException(
+      message := "Simple Resource Client has become invalid")
+    );
+    :- Need(input.value.Some?,
+      Types.SimpleResourceException(
+      message := "Input Value MUST be set")
+    );
+    var resource := new SimpleResource.SimpleResource(
+      input.value.value,
+      config
+     );
+     var result: GetResourcesOutput := GetResourcesOutput(
+      output := resource
+    );
+    return Success(result);  
+  }
   
 }
