TestModels/resources/src/Config.dfy
@@ -1,0 +1,23 @@
+// Copyright Amazon.com Inc. or its affiliates. All Rights Reserved.
+// SPDX-License-Identifier: Apache-2.0
+
+include "../Model/SimpleResourcesTypes.dfy"
+
+module Config {
+  import opened StandardLibrary
+  import Types = SimpleResourcesTypes    
+
+  datatype Config = Config(
+    nameonly name: string,
+    nameonly modified: bool := false
+  )
+
+  predicate method ValidInternalConfig?(config: Config)
+  {
+    && |config.name| > 0
+  }
+
+  function ModifiesInternalConfig(config: Config): set<object>
+  {{}}
+
+}
