TestModels/resources/src/SimpleResource.dfy
@@ -1,0 +1,75 @@
+// Copyright Amazon.com Inc. or its affiliates. All Rights Reserved.
+// SPDX-License-Identifier: Apache-2.0
+
+include "../Model/SimpleResourcesTypes.dfy"
+include "./Config.dfy"
+
+module SimpleResource {
+  import opened StandardLibrary
+  import opened Wrappers
+  import opened Config    
+  import Types = SimpleResourcesTypes    
+
+  class SimpleResource extends Types.ISimpleResource
+  {
+    const config: Config
+
+    predicate ValidState()
+      ensures ValidState() ==> History in Modifies
+    {
+      && History in Modifies
+      && ModifiesInternalConfig(config) <= Modifies
+      && History !in ModifiesInternalConfig(config)
+      && ValidInternalConfig?(config)
+    }
+
+    const value: string
+
+    constructor (
+      value: string,
+      config: Config
+    )
+      requires ValidInternalConfig?(config)
+      ensures this.value == value
+      ensures this.config == config
+      ensures ValidState() && fresh(History) && fresh(Modifies - ModifiesInternalConfig(config))
+    {
+      this.value := value;
+      this.config := config;
+
+      History := new Types.ISimpleResourceCallHistory();
+      Modifies := { History } + ModifiesInternalConfig(config);
+    }
+
+    predicate GetResourceDataEnsuresPublicly(
+      input: Types.GetResourceDataInput,
+      output: Result<Types.GetResourceDataOutput, Types.Error>
+    ) {true}
+
+    method GetResourceData'(
+      input: Types.GetResourceDataInput
+    ) returns (
+      output: Result<Types.GetResourceDataOutput, Types.Error>
+    )
+      requires ValidState()
+      modifies Modifies - {History}
+      decreases Modifies - {History}
+      ensures && ValidState()
+      ensures GetResourceDataEnsuresPublicly(input, output)
+      ensures unchanged(History)
+    {
+      var rtnString: string := if input.stringValue.Some? then
+        this.config.name + " " + input.stringValue.value
+      else
+        this.config.name;
+      var rtn: Types.GetResourceDataOutput := Types.GetResourceDataOutput(
+        blobValue := input.blobValue,
+        booleanValue := input.booleanValue,
+        stringValue := Option.Some(rtnString),
+        integerValue := input.integerValue,
+        longValue := input.longValue
+      );
+      return Success(rtn);  
+    }
+  }
+}
